move WriteAllocConditions into BBC.Varaibles

BlockCacheSystem/BlockCache.i.dfy
@@ -59,31 +59,29 @@ module BlockCache refines Transactable {
 
     | Unready
   {
-      // Conditions that will hold intermediately between writes and allocs
+    // Conditions that will hold intermediately between writes and allocs
+    predicate WriteAllocConditions()
+    {
+      && Ready?
+      && (forall loc | loc in ephemeralIndirectionTable.locs.Values :: ValidNodeLocation(loc))
+      && (forall r | r in ephemeralIndirectionTable.graph :: r <= ephemeralIndirectionTable.refUpperBound)
+      && AllLocationsForDifferentRefsDontOverlap(ephemeralIndirectionTable)
+    }
 
-      // predicate WriteAllocConditions()
-      // {
-      //   && Ready?
-      //   && (forall loc | loc in ephemeralIndirectionTable.locs.Values :: 
-      //         DiskLayout.ValidNodeLocation(loc))
-      //   && AllLocationsForDifferentRefsDontOverlap(ephemeralIndirectionTable)
-      // }
+    // predicate ChildrenConditions(succs: Option<seq<Reference>>)
+    // requires Ready?
+    // {
+    //   succs.Some? ==> (
+    //     && |succs.value| <= MaxNumChildren()
+    //     && IndirectionTable.SuccsValid(succs.value, ephemeralIndirectionTable.graph)
+    //   )
+    // }
 
-      // predicate ChildrenConditions(succs: Option<seq<Reference>>)
-      // requires Ready?
-      // {
-      //   succs.Some? ==> (
-      //     && |succs.value| <= MaxNumChildren()
-      //     && IT.IndirectionTable.SuccsValid(succs.value, s.ephemeralIndirectionTable.graph)
-      //   )
-      // }
-
-      function totalCacheSize() : int
-      requires Ready?
-      {
-        |cache| + |outstandingBlockReads|
-      }
-
+    function totalCacheSize() : int
+    requires Ready?
+    {
+      |cache| + |outstandingBlockReads|
+    }
   }
 
   predicate IsAllocated(s: Variables, ref: Reference)
@@ -103,6 +101,7 @@ module BlockCache refines Transactable {
   predicate WFCompleteIndirectionTable(indirectionTable: IndirectionTable)
   {
     && (forall loc | loc in indirectionTable.locs.Values :: ValidNodeLocation(loc))
+    && (forall r | r in indirectionTable.graph :: r <= indirectionTable.refUpperBound)
     && indirectionTable.graph.Keys == indirectionTable.locs.Keys
     && G.Root() in indirectionTable.graph
     && GraphClosed(indirectionTable.graph)
@@ -112,6 +111,7 @@ module BlockCache refines Transactable {
   predicate WFIndirectionTable(indirectionTable: IndirectionTable)
   {
     && (forall loc | loc in indirectionTable.locs.Values :: ValidNodeLocation(loc))
+    && (forall r | r in indirectionTable.graph :: r <= indirectionTable.refUpperBound)
     && indirectionTable.locs.Keys <= indirectionTable.graph.Keys
     && G.Root() in indirectionTable.graph
     && GraphClosed(indirectionTable.graph)
